src/program_proof/tulip/prelude.v
@@ -2,4 +2,6 @@ From Perennial.program_proof Require Export grove_prelude.
 From Perennial.program_logic Require Export atomic. (* prefer the ncfupd atomics *)
 From Perennial.program_proof.rsm Require Export big_sep.
 From Perennial.program_proof.rsm.pure Require Export
-  extend fin_maps list misc nat sets word quorum.
+  dual_lookup extend fin_maps largest_before list misc nat nonexpanding_merge sets vslice word.
+From Perennial.program_proof.tulip Require Export
+  action base res inv.
