src/program_proof/tulip/vos.sh
@@ -1,9 +1,23 @@
 #!/bin/bash
 
-dir='./src/program_proof/tulip'
+basedir='./src/program_proof/tulip'
+dir='.'
+prefix=''
 
-cd "$(dirname $0)"/../../../
-files=`find ${dir} -name "${1}*.v" ! -name "print_assumptions.v" | sed "s/\.v/\.vos/"`
+while getopts ":d:p:" option; do
+	case $option in
+		d)  dir=${OPTARG};;
+		p)  prefix=${OPTARG};;
+		\?) echo "Error: Invalid option"
+			exit;;
+	esac
+done
+
+echo "Checking files in: ${dir}"
+echo "Matching files with prefix: ${prefix}"
+
+cd ../../../
+files=`find ${basedir}/${dir} -name "${prefix}*.v" ! -name "print_assumptions.v" | sed "s/\.v/\.vos/"`
 if [[ -z ${files} ]]; then
     echo "No target files."
     exit 1
@@ -11,4 +25,4 @@ fi
 
 echo "Checking:"
 echo "`basename ${files}`"
-make -j8 ${files}
+make --ignore-errors -j8 ${files}
